nola/iris/csum.v
@@ -1,0 +1,46 @@
+(** * Utility for [csum] *)
+
+From nola Require Export prelude.
+From iris.algebra Require Export csum.
+
+(** Unfold [≡] over [csum] *)
+Lemma csum_equiv' {A B : ofe} {s s' : csum A B} :
+  s ≡ s' ↔
+    match s, s' with
+    | Cinl a, Cinl a' => a ≡ a'
+    | Cinr b, Cinr b' => b ≡ b'
+    | CsumBot, CsumBot => True
+    | _, _ => False
+    end.
+Proof. split; [by case|]. case: s; case: s'=>//= *; by f_equiv. Qed.
+(** Unfold [dist] over [csum] *)
+Lemma csum_dist' {A B : ofe} {n} {s s' : csum A B} :
+  s ≡{n}≡ s' ↔
+    match s, s' with
+    | Cinl a, Cinl a' => a ≡{n}≡ a'
+    | Cinr b, Cinr b' => b ≡{n}≡ b'
+    | CsumBot, CsumBot => True
+    | _, _ => False
+    end.
+Proof. split; [by case|]. case: s; case: s'=>//= *; by f_equiv. Qed.
+
+(** Unfold [≼] over [csum] *)
+Lemma csum_included' {A B : cmra} {s s' : csum A B} :
+  s ≼ s' ↔
+    match s, s' with
+    | _, CsumBot => True
+    | Cinl a, Cinl a' => a ≼ a'
+    | Cinr b, Cinr b' => b ≼ b'
+    | _, _ => False
+    end.
+Proof. rewrite csum_included. case: s; case: s'; naive_solver. Qed.
+(** Unfold [≼{_}] over [csum] *)
+Lemma csum_includedN {A B : cmra} {s s' : csum A B} {n} :
+  s ≼{n} s' ↔
+    match s, s' with
+    | _, CsumBot => True
+    | Cinl a, Cinl a' => a ≼{n} a'
+    | Cinr b, Cinr b' => b ≼{n} b'
+    | _, _ => False
+    end.
+Proof. rewrite csum_includedN. case: s; case: s'; naive_solver. Qed.
