nola/iris/list.v
@@ -9,12 +9,24 @@ Section big_cmra_opL.
   Context {C : ucmra}.
 
   (** For [∈] *)
-  Lemma big_cmra_opL_elem_of {A} {a al} (f : A → C) :
+  Lemma big_cmra_opL_included {A a al} (f : A → C) :
     a ∈ al → f a ≼ [^op list] a ∈ al, f a.
   Proof.
     elim: al=>/=. { by move=> /elem_of_nil. }
     move=> ?? IH /elem_of_cons[<-|/IH ?]; [done|]. by etrans.
   Qed.
+  Lemma core_id_included_big_cmra_opL' {A al} (f : A → C)
+    `{!∀ a, CoreId (f a)} {c} :
+    Forall (λ a, f a ≼ c) al → c ≡ ([^op list] a ∈ al, f a) ⋅ c.
+  Proof.
+    elim: al=>/=. { move=> _. by rewrite left_id. }
+    move=> ?? IH /Forall_cons[[cf eq] all]. rewrite -assoc -(IH all) eq assoc.
+    by rewrite -core_id_dup.
+  Qed.
+  Lemma core_id_included_big_cmra_opL {A al} (f : A → C)
+    `{!∀ a, CoreId (f a)} {c} :
+    Forall (λ a, f a ≼ c) al → ([^op list] a ∈ al, f a) ≼ c.
+  Proof. move=> /core_id_included_big_cmra_opL' ?. by exists c. Qed.
 
   (** [own] over [[^op list]] *)
   Lemma big_opL_own_2 `{!inG Σ C} {A} {γ al} (f : nat → A → C) :
