nola/iris/option.v
@@ -1,0 +1,33 @@
+(** * Utility for [option] *)
+
+From nola Require Export prelude.
+From iris.algebra Require Import cmra.
+
+(** Unfold [≡] over [option] *)
+Lemma option_equiv' {A : ofe} {o o' : option A} :
+  o ≡ o' ↔
+    match o, o' with
+    | Some a, Some a' => a ≡ a'
+    | None, None => True
+    | _, _ => False
+    end.
+Proof. split; [by case|]. case: o; case: o'=>// *. by f_equiv. Qed.
+(** Unfold [dist] over [option] *)
+Lemma option_dist' {A : ofe} {n} {o o' : option A} :
+  o ≡{n}≡ o' ↔
+    match o, o' with
+    | Some a, Some a' => a ≡{n}≡ a'
+    | None, None => True
+    | _, _ => False
+    end.
+Proof. split; [by case|]. case: o; case: o'=>// *. by f_equiv. Qed.
+
+(** Unfold [≼] over [option] *)
+Lemma option_included' {A : cmra} {o o' : option A} :
+  o ≼ o' ↔
+    match o, o' with
+    | None, _ => True
+    | Some a, Some a' => a ≡ a' ∨ a ≼ a'
+    | _, _ => False
+    end.
+Proof. rewrite option_included. case: o; case: o'; naive_solver. Qed.
